Esub.v
@@ -37,7 +37,7 @@ Qed.
 
 Definition app_esub : esub_i -> esub_j -> trm -> trm.
 intros es_i es_j t; left.
-exists (fun i => int (esub_conv_i es_i i) t) (fun j => tm (esub_conv_j es_j j) t).
+exists (fun i => int t (esub_conv_i es_i i)) (fun j => tm t (esub_conv_j es_j j)).
 do 4 red; intros. apply int_morph; try reflexivity.
  apply esub_conv_i_morph; trivial.
 
@@ -64,14 +64,14 @@ Defined.
 
 Definition sub_cons_i : trm -> esub_i -> esub_i.
 intros t es.
-exists (fun i => V.cons (int i t) (esub_conv_i es i)).
+exists (fun i => V.cons (int t i) (esub_conv_i es i)).
 do 2 red; intros. apply V.cons_morph; 
   [rewrite H; reflexivity| apply esub_conv_i_morph; trivial].
 Defined.
 
 Definition sub_cons_j : trm -> esub_j -> esub_j.
 intros t es.
-exists (fun j => I.cons (tm j t) (esub_conv_j es j)).
+exists (fun j => I.cons (tm t j) (esub_conv_j es j)).
 split; [|split]; intros.
  do 4 red; intros; rewrite H; trivial.
 
